\documentclass[10pt,a4paper]{article}

% PDF version and output
\pdfoutput=1        % force the execution of pdflatex
\pdfminorversion=7  % newest PDF version (1.7)

% Packages
\usepackage[utf8]{inputenc}
\usepackage{amsmath}
\usepackage{amsfonts}
\usepackage{amssymb}
\usepackage{geometry}
\usepackage{bookmark}   % loads hyperref

\geometry{
    a4paper,
    left=20mm,
    right=20mm,
    top=40mm,
    bottom=20mm,
}

% Informations
\author{Riccardo Finotello}
\title{Normal Ordering of a Free Boson}
\date{\today}

% Hyperref informations
\hypersetup
{
    pdftitle={Normal Ordering of a Free Boson},
    pdfsubject={Conformal Field Theory},
    pdfauthor={Riccardo Finotello},
    pdfkeywords={CFT, free boson, normal order, radial order},
    pdfstartview={FitH},
    pdfcreator={pdfTeX Tex Live 2015/Debian},
    pdfproducer={pdfLaTeX},
    pdfduplex={DuplexFlipLongEdge},
    pdflang={en-GB},
    pdfpagemode={UseOutlines},
    bookmarks={true},
    bookmarksopen={true},
    bookmarksnumbered={true},
    hidelinks
}

\begin{document}
    \pagenumbering{gobble}

    \maketitle

    Consider the boson field:
    \begin{equation*}
        X^{\mu}\left( z \right) = x^{\mu} + \alpha' p^{\mu} \ln\left( z \right)
        + i \sqrt{\frac{\alpha'}{2}} \sum\limits_{n \in \mathbb{Z}\backslash
        \left\lbrace 0 \right\rbrace} \frac{\alpha_n^{\mu}}{n} z^{-n},
    \end{equation*}
    and the commutation relations:
    \begin{align*}
        \left[ x^{\mu}, p^{\nu} \right] &= i \eta^{\mu \nu},
        \\
        \left[ \alpha_n^{\mu}, \alpha_m^{\nu} \right] &= n \eta^{\mu \nu}
        \delta_{n+m,0},
    \end{align*}
    where $\delta_{i,j}$ is the Kronecker delta.

    Then consider the radially ordered product between $X^{\mu}\left( z
    \right)$ and $X^{\nu}\left( w \right)$ ($\left| z \right| > \left| w
    \right|$):
    \begin{align*}
        &\mathrm{R}\left( X^{\mu}\left( z \right) X^{\nu}\left( w \right)
        \right) =
        \\
        &= \left( x^{\mu} + \alpha' p^{\mu} \ln\left( z \right) + i
        \sqrt{\frac{\alpha'}{2}} \sum\limits_{n \in \mathbb{Z}\backslash
        \left\lbrace 0 \right\rbrace} \frac{\alpha_n^{\mu}}{n} z^{-n} \right)
        \left( y^{\nu} + \alpha' q^{\nu} \ln\left( w \right) + i
        \sqrt{\frac{\alpha'}{2}} \sum\limits_{m \in \mathbb{Z}\backslash
        \left\lbrace 0 \right\rbrace} \frac{\alpha_m^{\nu}}{m} w^{-m} \right) =
        \\
        &= x^{\mu} y^{\nu} + \alpha' x^{\mu} q^{\nu} \ln\left( w \right) + i
        \sqrt{\frac{\alpha'}{2}} x^{\mu} \sum\limits_{m \in
        \mathbb{Z}\backslash \left\lbrace 0 \right\rbrace}
        \frac{\alpha^{\nu}_m}{m} w^{-m} +
        \\
        &+ \alpha' p^{\mu} y^{\nu} \ln\left( z \right) + \alpha'^2 p^{\mu}
        q^{\nu} \ln\left( z \right) \ln\left( w \right) + i \alpha'
        \sqrt{\frac{\alpha'}{2}} p^{\mu} \ln\left( z \right) \sum\limits_{m \in
        \mathbb{Z}\backslash \left\lbrace 0 \right\rbrace}
        \frac{\alpha^{\nu}_m}{m} w^{-m} +
        \\
        &+ i \sqrt{\frac{\alpha'}{2}} \sum\limits_{n \in \mathbb{Z}\backslash
        \left\lbrace 0 \right\rbrace} \frac{\alpha^{\mu}_n}{n} y^{\nu} z^{-n} +
        i \alpha' \sqrt{\frac{\alpha'}{2}}         \sum\limits_{n \in
        \mathbb{Z}\backslash \left\lbrace 0 \right\rbrace}
        \frac{\alpha^{\mu}_n}{n} q^{\nu} \ln\left( w \right) z^{-n} -
        \frac{\alpha'}{2} \sum\limits_{n \in \mathbb{Z}\backslash \left\lbrace
        0 \right\rbrace} \sum\limits_{m \in \mathbb{Z}\backslash \left\lbrace 0
        \right\rbrace} \frac{\alpha^{\mu}_n}{n} \frac{\alpha^{\nu}_m}{m} w^{-m}
        =
        \\
        &= \colon X^{\mu}\left( z \right) X^{\nu}\left( w \right) \colon -
        \frac{\alpha'}{2} \sum\limits_{n = 1}^{+\infty} \sum\limits_{m
        =1}^{+\infty} \frac{1}{nm} \left[ \alpha_n^{\mu}, \alpha_{-m}^{\nu}
        \right] z^{-n} w^m + \left[ p^{\mu}, y^{\nu} \right] \ln\left( z
        \right) =
        \\
        &= \colon X^{\mu}\left( z \right) X^{\nu}\left( w \right) \colon -
        \eta^{\mu\nu} \frac{\alpha'}{2} \sum\limits_{n = 1}^{+\infty}
        \frac{1}{n} \left( \frac{w}{z} \right)^n - i \eta^{\mu\nu} \ln\left( z
        \right) =
        \\
        &= \colon X^{\mu}\left( z \right) X^{\nu}\left( w \right) \colon -
        \eta^{\mu\nu} \frac{\alpha'}{2} \left( \ln\left( 1 - \frac{w}{z}
        \right) - \ln\left( z \right) \right) =
        \\
        &= \colon X^{\mu}\left( z \right) X^{\nu}\left( w \right) \colon -
        \eta^{\mu\nu} \frac{\alpha'}{2} \ln\left( z - w \right).
    \end{align*}

    Then, since:
    \begin{equation*}
        \mathrm{R}\left( X^{\mu}\left( z \right) X^{\nu}\left( w \right)
        \right) = \colon X^{\mu}\left( z \right) X^{\nu}\left( w \right) \colon
        + \left\langle X^{\mu}\left( z \right) X^{\nu}\left( w \right)
        \right\rangle,
    \end{equation*}
    we find:
    \begin{equation*}
        \left\langle X^{\mu}\left( z \right) X^{\nu}\left( w \right)
        \right\rangle = - \eta^{\mu\nu} \frac{\alpha'}{2} \ln\left( z - w
        \right).
    \end{equation*}

\end{document}
