\documentclass[10pt,a4paper]{article}

% PDF version and output
\pdfoutput=1        % force the execution of pdflatex
\pdfminorversion=7  % newest PDF version (1.7)

% Packages
\usepackage[utf8]{inputenc}
\usepackage{amsmath}
\usepackage{amsfonts}
\usepackage{amssymb}
\usepackage{geometry}
\usepackage{bookmark}   % loads hyperref

\geometry{
    a4paper,
    left=20mm,
    right=20mm,
    top=40mm,
    bottom=20mm,
}

% Informations
\author{Riccardo Finotello}
\title{Operator Product Expansion of a Vertex Operator}
\date{\today}

% Hyperref informations
\hypersetup
{
    pdftitle={Operator Product Expansion of a Vertex Operator},
    pdfsubject={Conformal Field Theory},
    pdfauthor={Riccardo Finotello},
    pdfkeywords={CFT, free boson, normal order, radial order},
    pdfstartview={FitH},
    pdfcreator={pdfTeX Tex Live 2015/Debian},
    pdfproducer={pdfLaTeX},
    pdfduplex={DuplexFlipLongEdge},
    pdflang={en-GB},
    pdfpagemode={UseOutlines},
    bookmarks={true},
    bookmarksopen={true},
    bookmarksnumbered={true},
    hidelinks
}

\begin{document}
    \pagenumbering{gobble}

    \maketitle

    Consider:
    \begin{align*}
        \left\langle X^{\alpha}\left( z \right) X^{\beta}\left( w \right)
        \right\rangle &= - \eta^{\alpha\beta} \ln\left( z - w \right),
        \\
        \left\langle \partial_z X^{\alpha}\left( z \right) X^{\beta}\left( w
        \right) \right\rangle &= - \eta^{\alpha\beta} \frac{1}{z-w},
        \\
        \left\langle \partial_z X^{\alpha}\left( z \right) \partial_w
        X^{\beta}\left( w \right) \right\rangle &= - \eta^{\alpha\beta}
        \frac{1}{\left( z - w \right)^2}.
    \end{align*}

    Then:
    \begin{align*}
        \partial_z X^{\alpha}\left( z \right) \colon e^{i k_{\beta}
        X^{\beta}\left( w \right)} \colon &= \partial_z X^{\alpha}\left( z
        \right) \colon 1 \colon + \partial_z X^{\alpha}\left( z \right) \left(
        i k_{\beta} \right) \colon X^{\beta}\left( w \right) \colon +
        \\
        &+ \frac{1}{2} \partial_z X^{\alpha}\left( z \right) \left( i^2
        k_{\beta} k_{\gamma} \right) \colon X^{\beta}\left( w \right)
        X^{\gamma}\left( w \right) \colon + \ldots =
        \\
        &= \partial_z X^{\alpha}\left( z \right) \colon 1 \colon + i k_{\beta}
        \left\langle \partial_z X^{\alpha}\left( z \right) X^{\beta}\left( w
        \right) \right\rangle -
        \\
        &- \frac{1}{2} k_{\beta} k_{\gamma} \left( \left\langle \partial_z
        X^{\alpha}\left( z \right) X^{\beta}\left( w \right) \right\rangle
        X^{\gamma}\left( w \right) + \left\langle \partial_z X^{\alpha}\left( z
        \right) X^{\gamma}\left( w \right) \right\rangle X^{\beta}\left( w
        \right) \right) + \ldots =
        \\
        &= \partial_z X^{\alpha}\left( z \right) + \frac{i k^{\alpha}}{z - w} -
        \frac{k^{\alpha}}{z - w} k \cdot X\left( w \right) + \ldots =
        \\
        &= \frac{i k^{\alpha}}{z - w} \colon \sum\limits_{n = 0}^{+\infty}
        \frac{\left( i k \cdot X\left( w \right) \right)^n}{n!} =
        \\
        &= \frac{i k^{\alpha}}{z - w} \colon e^{i k \cdot X\left( w \right)}
        \colon.
    \end{align*}

    Therefore:
    \begin{equation*}
        \partial_z X^{\alpha}\left( z \right) \colon e^{i k \cdot X\left( w
        \right)} \colon = \frac{i k^{\alpha}}{z - w} \colon e^{i k \cdot
        X\left( w \right)} \colon.
    \end{equation*}
\end{document}
