\documentclass[10pt,a4paper]{article}

% PDF version and output
\pdfoutput=1        % force the execution of pdflatex
\pdfminorversion=7  % newest PDF version (1.7)

% Packages
\usepackage[utf8]{inputenc}
\usepackage{amsmath}
\usepackage{amsfonts}
\usepackage{amssymb}
\usepackage{geometry}
\usepackage{bookmark}   % loads hyperref

\geometry{
    a4paper,
    left=20mm,
    right=20mm,
    top=40mm,
    bottom=20mm,
}

% Informations
\author{Riccardo Finotello}
\title{Normal Ordering of a Free Boson}
\date{\today}

% Hyperref informations
\hypersetup
{
    pdftitle={Normal Ordering of a Free Boson},
    pdfsubject={Conformal Field Theory},
    pdfauthor={Riccardo Finotello},
    pdfkeywords={CFT, free boson, normal order, radial order},
    pdfstartview={FitH},
    pdfcreator={pdfTeX Tex Live 2015/Debian},
    pdfproducer={pdfLaTeX},
    pdfduplex={DuplexFlipLongEdge},
    pdflang={en-GB},
    pdfpagemode={UseOutlines},
    bookmarks={true},
    bookmarksopen={true},
    bookmarksnumbered={true},
    hidelinks
}

\begin{document}
    \pagenumbering{gobble}

    \maketitle

    Consider the holomorphic field $\partial_z X\left( z \right)$ (conformal
    weight $\left( 1, 0 \right)$):
    \begin{align*}
        \partial_z X\left( z \right) &= -i \sqrt{\frac{\alpha'}{2}}
        \sum\limits_{n \in \mathbb{Z}} \alpha_n z^{-n-1} =
        \\
        &= -i \sqrt{\frac{\alpha'}{2}} \sum\limits_{n = 0}^{+\infty} \left(
        \alpha_n z^{-n-1} + \alpha_{-n-1} z^n \right),
    \end{align*}
    and the commutation relation:
    \begin{equation*}
        \left[ \alpha_n, \alpha_m \right] = n \delta_{n+m,0},
    \end{equation*}
    where $\delta_{i,j}$ is the Kronecker delta.

    Then the radially ordered product between $\partial_z X\left( z \right)$
    and $\partial_w X\left( w \right)$ ($\left| z \right| > \left| w \right|$)
    is:
    \begin{align*}
        &\mathrm{R}\left( \partial_z X\left( z \right) \partial_w X\left( w
        \right) \right) =
        \\
        &= -\frac{\alpha'}{2} \sum\limits_{n = 0}^{+\infty} \sum\limits_{m =
        0}^{+\infty} \left( \alpha_n \alpha_m z^{-n-1} w^{-m-1} + \right.
        \\
        &\left. + \alpha_n \alpha_{-m-1} z^{-n-1}
        w^m + \alpha_{-n-1} \alpha_m z^n w^{-m-1} + \alpha_{-n-1} \alpha_{-m-1}
        z^n w^m \right) =
        \\
        &= \colon \partial_z X\left( z \right) \partial_w X\left( w \right)
        \colon - \frac{\alpha'}{2} \sum\limits_{n = 0}^{+\infty} \sum\limits_{m
        = 0}^{+\infty} \left[ \alpha_n, \alpha_{-m-1} \right] z^{-n-1} w^m =
        \\
        &= \colon \partial_z X\left( z \right) \partial_w X\left( w \right)
        \colon - \frac{\alpha'}{2} \sum\limits_{n = 0}^{+\infty} n z^{-n-1}
        w^{n-1} =
        \\
        &= \colon \partial_z X\left( z \right) \partial_w X\left( w \right)
        \colon + \frac{1}{zw} \frac{\alpha'}{2} \sum\limits_{n = 1}^{+\infty} n
        \left( \frac{w}{z} \right)^n =
        \\
        &= \colon \partial_z X\left( z \right) \partial_w X\left( w \right)
        \colon - \frac{1}{zw} \frac{\alpha'}{2} \frac{ w / z }{\left( 1 - w / z
        \right)^2} =
        \\
        &= \colon \partial_z X\left( z \right) \partial_w X\left( w \right)
        \colon - \frac{\alpha'}{2} \frac{1}{\left( z - w \right)^2}.
    \end{align*}

    Then, since:
    \begin{equation*}
        \mathrm{R}\left( \partial_z X\left( z \right) \partial_w X\left( w
        \right) \right) = \colon \partial_z X\left( z \right) \partial_w X\left(
        w \right) \colon + \left\langle \partial_z X\left( z \right) \partial_w
        X\left( w \right) \right\rangle,
    \end{equation*}
    we find:
    \begin{equation*}
        \left\langle \partial_z X\left( z \right) \partial_w X\left( w \right)
        \right\rangle = - \frac{\alpha'}{2} \frac{1}{\left( z - w \right)^2}.
    \end{equation*}

    Then:
    \begin{align*}
        T\left( z \right) &= \frac{2}{\alpha'} \colon \partial_z X\left( z
        \right) \partial_z X\left( z \right) \colon =
        \\
        &= \lim\limits_{w \to z} \left[ \frac{2}{\alpha'} \mathrm{R}\left(
        \partial_z X\left( w \right) \partial_z X\left( z \right) \right) +
        \frac{1}{\left( w - z \right)^2} \right].
    \end{align*}

\end{document}
